Cleaner MoSel

cfrontend/MoSel.v
@@ -152,23 +152,24 @@ Module gensym.
     * simpl. do 2 f_equal. apply functional_extensionality. intro. apply m.
   Qed.
 
-  Definition fresh (ty : type) (s: generator) : ident * generator :=
-    let h := gen_trail s in
-    let n := gen_next s in
-    (n, mkgenerator  (Pos.succ n) ((n,ty) :: h)).
+  Fixpoint eval {X} (m : mon X) : generator -> res (generator * X) :=
+  match m with
+  | ret v => fun s => OK (s, v)
+  | errorOp e => fun s => Error e
+  | gensymOp ty f =>
+    fun s =>
+      let h := gen_trail s in
+      let n := gen_next s in
+      eval (f n) (mkgenerator (Pos.succ n) ((n,ty) :: h))
+  end.
 
-  Fixpoint run {X} (m : mon X) : generator -> res (generator * X) :=
-    match m with
-    | ret v => fun s => OK (s, v)
-    | errorOp e => fun s => Error e
-    | gensymOp t f =>
-      fun s =>
-        let (i,s') := fresh t s in
-        run (f i) s'
-    end.
+Definition run {X} (m: mon X): res X :=
+  match eval m initial_state with
+  | OK (_, v) => OK v
+  | Error e => Error e
+  end.
 
 End gensym.
-
 
 Module weakestpre_gensym.
   Export gensym.
@@ -279,6 +280,7 @@ Proof. auto. Qed.
 End weakestpre_gensym.
 
 Module adequacy.
+  Import Errors.
   Export weakestpre_gensym.
 
   Definition inject n := List.map Pos.of_nat (seq 1 (pred (Pos.to_nat n))).
@@ -305,7 +307,7 @@ Module adequacy.
 
   Lemma adequacy_wp {X} : forall (e : mon X) (Q : X -> iProp) (s s' : generator) v,
       (heap_ctx (inject (gen_next s)) ⊢ wp e Q) ->
-      run e s = Errors.OK (s', v) ->
+      eval e s = Errors.OK (s', v) ->
       (Q v) () (inject (gen_next s')).
   Proof.
     fix e 1.
@@ -322,13 +324,13 @@ Module adequacy.
 
   Lemma adequacy_init {X} : forall (e : mon X) (Q : X -> iProp) s' v,
       (⊢ wp e Q) ->
-      run e initial_state = Errors.OK (s', v) ->
+      eval e initial_state = Errors.OK (s', v) ->
       (Q v) () (inject (gen_next s')).
   Proof. intros. eapply adequacy_wp; eauto. auto. Qed.
 
-  Lemma adequacy {X} : forall (e : mon X) (Q : X -> iProp) s v s' H,
+  Lemma adequacy_core {X} : forall (e : mon X) (Q : X -> iProp) s v s' H,
       (heap_ctx (inject (gen_next s)) ⊢ H) -> (⊢ {{ H }} e {{ v; Q v }}) ->
-      run e s = Errors.OK (s', v) ->
+      eval e s = Errors.OK (s', v) ->
       (Q v) () (inject (gen_next s')).
   Proof.
     intros. eapply adequacy_wp; eauto. iIntros "HA". iDestruct (H0 with "HA") as "HA".
@@ -337,7 +339,7 @@ Module adequacy.
 
   Lemma adequacy_triple_init {X} : forall (e : mon X) (Q : X -> iProp) v s' H,
       (⊢ H) -> (⊢ {{ H }} e {{ v; Q v }}) ->
-      run e initial_state = Errors.OK (s', v) ->
+      eval e initial_state = Errors.OK (s', v) ->
       (Q v) () (inject (gen_next s')).
   Proof.
     intros. eapply adequacy_init; eauto. iApply H1; eauto.
@@ -345,7 +347,7 @@ Module adequacy.
 
   Lemma adequacy_wp_pure {X} : forall (e : mon X) (Q : X -> Prop) s v s',
       (heap_ctx (inject (gen_next s)) ⊢ wp e (fun v =>  ⌜Q v⌝)) ->
-      run e s = Errors.OK (s', v) ->
+      eval e s = Errors.OK (s', v) ->
       Q v.
   Proof.
     intros. apply (soundness_pure (inject (gen_next s'))). iApply completeness.
@@ -354,20 +356,33 @@ Module adequacy.
 
   Lemma adequacy_pure {X} : forall (e : mon X) (Q : X -> Prop) s v s' H,
       (heap_ctx (inject (gen_next s)) ⊢ H) -> (⊢ {{ H }} e {{ v; ⌜ Q v ⌝}}) ->
-      run e s = Errors.OK (s', v) ->
+      eval e s = Errors.OK (s', v) ->
       Q v.
   Proof.
     intros. eapply adequacy_wp_pure; eauto. iIntros "HA". iDestruct (H0 with "HA") as "HA".
     iDestruct (H1 with "HA") as "$".
   Qed.
 
-  Lemma adequacy_pure_init {X} : forall (e : mon X) (Q : X -> Prop) v s' H,
-      (⊢ H) -> (⊢ {{ H }} e {{ v; ⌜ Q v ⌝}}) ->
-      run e initial_state = Errors.OK (s', v) ->
-      Q v.
+  Section Adequacy.
+  Variable X: Type.
+  Implicit Type m: mon X.
+  Implicit Type P: iProp.
+  Implicit Type Q: X -> Prop.
+  Implicit Type v: X.
+
+  Lemma adequacy: forall m P Q v,
+      (⊢ P) -> (⊢ {{ P }} m {{ v; ⌜ Q v ⌝}}) ->
+      run m = OK v -> Q v.
   Proof.
-    intros. eapply adequacy_pure; eauto.
-    iIntros "_". iApply H1; auto.
+    intros m.
+    unfold run. intros.
+    destruct (eval m initial_state) eqn:H2; try inversion H1.
+    destruct p. inversion H1; subst.
+    eapply adequacy_pure; eauto.
+    iIntros "_".
+    iApply H0. iApply H.
   Qed.
+
+  End Adequacy.
 
 End adequacy.
